testAvl.v
@@ -1,0 +1,98 @@
+Set Warnings "-deprecated-hint-without-locality,-implicit-core-hint-db".
+
+(** I wanted to use QuickChick to test AVL operations preserve
+    all kinds of proerties. But after I write down all the proofs
+    of decidability of these properties, I realised I can not
+    test these propositions since we can not prove whether they hold
+    or not automatically even though they are decidable. So if we want to
+    test these properties, we have to define the function versions of
+    all these proerties and prove they are equal to the prosition
+    versions. Therefore, the following code is not really useful. *)
+
+From BST Require Import project.
+Require Import List. Import ListNotations.
+From QuickChick Require Import QuickChick. Import QcNotation.
+Require Import ssreflect ssrbool.
+Require Import String.
+
+Hint Constructors project.all.
+Hint Constructors sorted.
+
+Local Open Scope string_scope.
+#[local] Instance showTree : Show tree :=
+  {| show := let fix aux t :=
+       match t with
+         | leaf => "leaf"
+         | node x lhs rhs =>
+             "node (" ++ show x ++ ") ("
+                      ++ aux lhs ++ ") ("
+                      ++ aux rhs ++ ")"
+       end
+     in aux
+  |}.
+Local Close Scope string_scope.
+
+Fixpoint genTreeSized (sz : nat) (g : G nat) : G tree :=
+  match sz with
+    | O => ret leaf
+    | S sz' =>
+        freq [ (1, ret leaf) ;
+               (sz, liftM3 node g (genTreeSized sz' g)
+                                  (genTreeSized sz' g))
+             ]
+  end.
+
+Fixpoint shrinkTreeAux (s : nat -> list nat) (t : tree) : list tree :=
+  match t with
+    | leaf => []
+    | node x l r => [l] ++ [r] ++
+                    map (fun x' => node x' l r) (s x) ++
+                    map (fun l' => node x l' r) (shrinkTreeAux s l) ++
+                    map (fun r' => node x l r') (shrinkTreeAux s r)
+  end.
+
+#[local] Instance dec_all_less : forall n t, Dec (project.all (fun x => x < n) t).
+Proof.
+  constructor. induction t.
+  - unfold decidable. left; auto.
+  - assert (Hlt: decidable (n0 < n)) by apply Compare_dec.lt_dec.
+    destruct Hlt; destruct IHt1; destruct IHt2; unfold decidable;
+    (* One thing don't like about coq: can't do something with some specific clauses I want *)
+    try solve [left; auto];
+    solve [right; intro H; inversion H; contradiction].
+Defined.
+
+#[local] Instance dec_all_greater : forall n t, Dec (project.all (fun x => n < x) t).
+Proof.
+  constructor. induction t.
+  - unfold decidable. left; auto.
+  - assert (Hlt: decidable (n < n0)) by apply Compare_dec.lt_dec.
+    destruct Hlt; destruct IHt1; destruct IHt2; unfold decidable;
+    try solve [left; auto];
+    solve [right; intro H; inversion H; contradiction].
+Defined.
+
+#[local] Instance dec_sorted : forall t, Dec (sorted t).
+Proof.
+  constructor. induction t.
+  - unfold decidable. left; auto.
+  - assert (Hall1: decidable (project.all (fun x => x < n) t1)) by apply dec_all_less.
+    assert (Hall2: decidable (project.all (fun x => n < x) t2)) by apply dec_all_greater.
+    destruct IHt1; destruct IHt2; destruct Hall1; destruct Hall2; unfold decidable;
+    try solve [left; auto];
+    solve [right; intro H; inversion H; contradiction].
+Defined.
+
+#[local] Instance dec_balancedF : forall t, Dec (AVL.balanced t = true).
+Proof. intros. dec_eq. Defined.
+
+#[local] Instance dec_balanced : forall t, Dec (AVL.balancedP t).
+Proof.
+  intros.
+  assert (H: decidable (AVL.balanced t = true)) by apply dec_balancedF.
+  destruct H as [H | H]; rewrite <- (AVL.balanced_prop t) in H;
+  constructor; unfold decidable; auto.
+Qed.
+
+#[local] Instance dec_avl : forall t, Dec (AVL.avl t).
+Proof. constructor. unfold AVL.avl. Fail apply Decidable.dec_and. Admitted.
